floyd/local2ptree.v
@@ -1238,8 +1238,8 @@ Fixpoint msubst_eval_expr {cs: compspecs} (T1: PTree.t val) (T2: PTree.t vardesc
 
   | Ederef a ty => msubst_eval_expr T1 T2 a
   | Efield a i ty => option_map (eval_field (typeof a) i) (msubst_eval_lvalue T1 T2 a)
-  | Esizeof t _ => Some (Vint (Int.repr (sizeof cenv_cs t)))
-  | Ealignof t _ => Some (Vint (Int.repr (alignof cenv_cs t)))
+  | Esizeof t _ => Some (Vint (Int.repr (sizeof t)))
+  | Ealignof t _ => Some (Vint (Int.repr (alignof t)))
   end
   with msubst_eval_lvalue {cs: compspecs} (T1: PTree.t val) (T2: PTree.t vardesc) (e: Clight.expr) : option val := 
   match e with 
