sha/verif_hmacNK_cleanup.v
@@ -20,14 +20,14 @@ name ctx' _ctx.
 unfold hmacstate_PostFinal, hmac_relate_PostFinal.
 Intros hst.
 Time assert_PROP (field_compatible t_struct_hmac_ctx_st [] c) as FCc by entailer!. (*8.7*)
-forward_call (Tsh, c, sizeof (@cenv_cs CompSpecs) t_struct_hmac_ctx_st, Int.zero).
+forward_call (Tsh, c, sizeof t_struct_hmac_ctx_st, Int.zero).
   { eapply derives_trans. apply data_at_data_at_.
     rewrite <- memory_block_data_at_; try reflexivity. cancel.
     trivial. }
 Intros rv; subst rv.
 subst POSTCONDITION; unfold abbreviate.
-pose proof (sizeof_pos cenv_cs t_struct_hmac_ctx_st).
-forget (sizeof cenv_cs t_struct_hmac_ctx_st) as NN.
+pose proof (sizeof_pos t_struct_hmac_ctx_st).
+forget (sizeof t_struct_hmac_ctx_st) as NN.
 forward.
 unfold data_block. simpl. rewrite Zlength_list_repeat by omega.
 rewrite !map_list_repeat.
@@ -46,14 +46,14 @@ Intros key.
 unfold hmacstate_PreInitNull, hmac_relate_PreInitNull.
 Intros hst X.
 Time assert_PROP (field_compatible t_struct_hmac_ctx_st [] c) as FCc by entailer!. (*8.9*)
-forward_call (Tsh, c, sizeof (@cenv_cs CompSpecs) t_struct_hmac_ctx_st, Int.zero).
+forward_call (Tsh, c, sizeof t_struct_hmac_ctx_st, Int.zero).
   { eapply derives_trans. apply data_at_data_at_.
     rewrite <- memory_block_data_at_; try reflexivity. cancel.
     trivial. }
 Intros rv; subst rv.
 subst POSTCONDITION; unfold abbreviate.
-pose proof (sizeof_pos cenv_cs t_struct_hmac_ctx_st).
-forget (sizeof cenv_cs t_struct_hmac_ctx_st) as NN.
+pose proof (sizeof_pos t_struct_hmac_ctx_st).
+forget (sizeof t_struct_hmac_ctx_st) as NN.
 forward.
 unfold data_block. simpl. rewrite Zlength_list_repeat by omega.
 rewrite !map_list_repeat.
